tutorial/windows_build.bat
@@ -1,0 +1,38 @@
+@SET coqc="C:\Coq\bin\coqc.exe"
+@SET coqdoc="C:\Coq\bin\coqdoc.exe"
+@IF NOT EXIST %coqc% (
+  @ECHO Error: %coqc% does not exist.
+  @ECHO Please edit the first line of this batch file to point to coqc.exe.
+  @GOTO ErrorExit
+)
+@IF NOT EXIST %coqdoc% (
+  @ECHO Error: %coqdoc% does not exist.
+  @ECHO Please edit the second line of this batch file to point to coqdoc.exe.
+  @GOTO ErrorExit
+)
+@SET coqc=%coqc% -R .. Picinae
+@SET coqdoc=%coqdoc% -R .. Picinae
+%coqc% AbsAndPracs.v
+%coqdoc% AbsAndPracs.v
+@IF ERRORLEVEL 1 GOTO :ErrorExit
+%coqc% BasicLoops.v
+%coqdoc% BasicLoops.v
+@IF ERRORLEVEL 1 GOTO :ErrorExit
+%coqc% Basics.v
+%coqdoc% Basics.v
+@IF ERRORLEVEL 1 GOTO :ErrorExit
+%coqc% Foundation.v
+%coqdoc% Foundation.v
+@IF ERRORLEVEL 1 GOTO :ErrorExit
+%coqc% PicinaeAuto.v
+%coqdoc% PicinaeAuto.v
+@IF ERRORLEVEL 1 GOTO :ErrorExit
+%coqc% Preface.v
+%coqdoc% Preface.v
+@IF ERRORLEVEL 1 GOTO :ErrorExit
+@ECHO Picinae build succeeded!
+@GOTO Done
+:ErrorExit
+@ECHO Script failed with errors. Aborting.
+:Done
+@PAUSE
